opentheory/examples/byte-word.ml
@@ -1,0 +1,253 @@
+(* byte *)
+
+(* byte-def *)
+
+new_constant ("byte_size", `:num`);;
+
+let byte_size_def = new_axiom
+  `byte_size = 2 EXP byte_width`;;
+
+let byte_size_nonzero = new_axiom
+  `~(byte_size = 0)`;;
+
+(* byte *)
+
+(* byte-mod *)
+
+let mod_lt_byte_size = new_axiom
+  `!n. n < byte_size ==> n MOD byte_size = n`;;
+
+let lt_mod_byte_size = new_axiom
+  `!n. n MOD byte_size < byte_size`;;
+
+let mod_mod_refl_byte_size = new_axiom
+  `!n. n MOD byte_size MOD byte_size = n MOD byte_size`;;
+
+let mod_add_mod_byte_size = new_axiom
+  `!m n. (m MOD byte_size + n MOD byte_size) MOD byte_size = (m + n) MOD byte_size`;;
+
+let mod_mult_mod2_byte_size = new_axiom
+  `!m n. (m MOD byte_size * n MOD byte_size) MOD byte_size = (m * n) MOD byte_size`;;
+
+(* byte-def *)
+
+new_type ("byte",0);;
+
+new_constant ("num_to_byte", `:num -> byte`);;
+
+new_constant ("byte_to_num", `:byte -> num`);;
+
+let byte_to_num_to_byte = new_axiom
+  `!x. num_to_byte (byte_to_num x) = x`;;
+
+let num_to_byte_inj = new_axiom
+   `!x y.
+      x < byte_size /\ y < byte_size /\ num_to_byte x = num_to_byte y ==>
+      x = y`;;
+
+let num_to_byte_to_num = new_axiom
+  `!x. byte_to_num (num_to_byte x) = x MOD byte_size`;;
+
+new_constant ("byte_add", `:byte -> byte -> byte`);;
+
+let num_to_byte_add = new_axiom
+  `!x1 y1.
+     num_to_byte (x1 + y1) =
+     byte_add (num_to_byte x1) (num_to_byte y1)`;;
+
+new_constant ("byte_mult", `:byte -> byte -> byte`);;
+
+let num_to_byte_mult = new_axiom
+  `!x1 y1.
+     num_to_byte (x1 * y1) =
+     byte_mult (num_to_byte x1) (num_to_byte y1)`;;
+
+new_constant ("byte_neg", `:byte -> byte`);;
+
+let byte_neg_def = new_axiom
+  `!x. byte_neg x = num_to_byte (byte_size - byte_to_num x)`;;
+
+new_constant ("byte_sub", `:byte -> byte -> byte`);;
+
+let byte_sub_def = new_axiom
+  `!x y. byte_sub x y = byte_add x (byte_neg y)`;;
+
+new_constant ("byte_le", `:byte -> byte -> bool`);;
+
+let byte_le_def = new_axiom
+  `!x y. byte_le x y = byte_to_num x <= byte_to_num y`;;
+
+new_constant ("byte_lt", `:byte -> byte -> bool`);;
+
+let byte_lt_def = new_axiom
+  `!x y. byte_lt x y = ~(byte_le y x)`;;
+
+(* byte-thm *)
+
+let byte_to_num_inj = new_axiom
+  `!x y. byte_to_num x = byte_to_num y ==> x = y`;;
+
+let num_to_byte_eq = new_axiom
+   `!x y.
+      num_to_byte x = num_to_byte y <=> x MOD byte_size = y MOD byte_size`;;
+
+let byte_to_num_bound = new_axiom
+  `!x. byte_to_num x < byte_size`;;
+
+let byte_to_num_div_bound = new_axiom
+  `!x. byte_to_num x DIV byte_size = 0`;;
+
+let byte_add_to_num = new_axiom
+   `!x y.
+      byte_to_num (byte_add x y) =
+      (byte_to_num x + byte_to_num y) MOD byte_size`;;
+
+(* byte-bits-def *)
+
+new_constant ("byte_shl", `:byte -> num -> byte`);;
+
+let byte_shl_def = new_axiom
+  `!w n. byte_shl w n = num_to_byte ((2 EXP n) * byte_to_num w)`;;
+
+new_constant ("byte_shr", `:byte -> num -> byte`);;
+
+let byte_shr_def = new_axiom
+  `!w n. byte_shr w n = num_to_byte (byte_to_num w DIV (2 EXP n))`;;
+
+new_constant ("byte_bit", `:byte -> num -> bool`);;
+
+let byte_bit_def = new_axiom
+  `!w n. byte_bit w n = ODD (byte_to_num (byte_shr w n))`;;
+
+new_constant ("byte_to_list", `:byte -> bool list`);;
+
+let byte_to_list_def = new_axiom
+  `!w. byte_to_list w = MAP (byte_bit w) (interval 0 byte_width)`;;
+
+new_constant ("list_to_byte", `:bool list -> byte`);;
+
+let list_to_byte_def = new_axiom
+  `(list_to_byte [] = num_to_byte 0) /\
+   (!h t.
+      list_to_byte (CONS h t) =
+      if h then byte_add (byte_shl (list_to_byte t) 1) (num_to_byte 1)
+      else byte_shl (list_to_byte t) 1)`;;
+
+new_constant ("is_byte_list", `:bool list -> bool`);;
+
+let is_byte_list_def = new_axiom
+  `!l. is_byte_list (l : bool list) <=> LENGTH l = byte_width`;;
+
+new_constant ("byte_and", `:byte -> byte -> byte`);;
+
+let byte_and_def = new_axiom
+  `!w1 w2.
+     byte_and w1 w2 =
+     list_to_byte (zipwith ( /\ ) (byte_to_list w1) (byte_to_list w2))`;;
+
+new_constant ("byte_or", `:byte -> byte -> byte`);;
+
+let byte_or_def = new_axiom
+  `!w1 w2.
+     byte_or w1 w2 =
+     list_to_byte (zipwith ( \/ ) (byte_to_list w1) (byte_to_list w2))`;;
+
+new_constant ("byte_not", `:byte -> byte`);;
+
+let byte_not_def = new_axiom
+  `!w. byte_not w = list_to_byte (MAP (~) (byte_to_list w))`;;
+
+(* byte-bits-thm *)
+
+let length_byte_to_list = new_axiom
+  `!w. LENGTH (byte_to_list w) = byte_width`;;
+
+let is_byte_to_list = new_axiom
+  `!w. is_byte_list (byte_to_list w)`;;
+
+let byte_bit_div = new_axiom
+  `!w n. byte_bit w n = ODD (byte_to_num w DIV (2 EXP n))`;;
+
+let nil_to_byte_to_num = new_axiom
+  `byte_to_num (list_to_byte []) = 0`;;
+
+let cons_to_byte_to_num = new_axiom
+   `!h t.
+      byte_to_num (list_to_byte (CONS h t)) =
+      (2 * byte_to_num (list_to_byte t) + (if h then 1 else 0)) MOD byte_size`;;
+
+let list_to_byte_to_num_bound = new_axiom
+  `!l. byte_to_num (list_to_byte l) < 2 EXP (LENGTH l)`;;
+
+let list_to_byte_to_num_bound_suc = new_axiom
+  `!l. 2 * byte_to_num (list_to_byte l) + 1 < 2 EXP (SUC (LENGTH l))`;;
+
+let cons_to_byte_to_num_bound = new_axiom
+   `!h t.
+      2 * byte_to_num (list_to_byte t) + (if h then 1 else 0) <
+      2 EXP SUC (LENGTH t)`;;
+
+let byte_to_list_to_byte = new_axiom
+  `!w. list_to_byte (byte_to_list w) = w`;;
+
+let byte_to_list_inj = new_axiom
+  `!w1 w2. byte_to_list w1 = byte_to_list w2 ==> w1 = w2`;;
+
+let list_to_byte_bit = new_axiom
+   `!l n.
+      byte_bit (list_to_byte l) n =
+      (n < byte_width /\ n < LENGTH l /\ EL n l)`;;
+
+let short_list_to_byte_to_list = new_axiom
+   `!l.
+      LENGTH l <= byte_width ==>
+      byte_to_list (list_to_byte l) =
+      APPEND l (REPLICATE (byte_width - LENGTH l) F)`;;
+
+let long_list_to_byte_to_list = new_axiom
+   `!l.
+      byte_width <= LENGTH l ==>
+      byte_to_list (list_to_byte l) = take byte_width l`;;
+
+let list_to_byte_to_list_eq = new_axiom
+   `!l.
+      byte_to_list (list_to_byte l) =
+      if LENGTH l <= byte_width then
+        APPEND l (REPLICATE (byte_width - LENGTH l) F)
+      else
+        take byte_width l`;;
+
+let list_to_byte_to_list = new_axiom
+  `!l. LENGTH l = byte_width <=> byte_to_list (list_to_byte l) = l`;;
+
+let byte_shl_list = new_axiom
+   `!l n.
+      byte_shl (list_to_byte l) n =
+      list_to_byte (APPEND (REPLICATE n F) l)`;;
+
+let short_byte_shr_list = new_axiom
+   `!l n.
+      LENGTH l <= byte_width ==>
+      byte_shr (list_to_byte l) n =
+      (if LENGTH l <= n then list_to_byte []
+       else list_to_byte (drop n l))`;;
+
+let long_byte_shr_list = new_axiom
+   `!l n.
+      byte_width <= LENGTH l ==>
+      byte_shr (list_to_byte l) n =
+      if byte_width <= n then list_to_byte []
+      else list_to_byte (drop n (take byte_width l))`;;
+
+let byte_shr_list = new_axiom
+   `!l n.
+      byte_shr (list_to_byte l) n =
+      (if LENGTH l <= byte_width then
+         if LENGTH l <= n then list_to_byte []
+         else list_to_byte (drop n l)
+       else
+         if byte_width <= n then list_to_byte []
+         else list_to_byte (drop n (take byte_width l)))`;;
+
+let byte_eq_bits = new_axiom
+  `!w1 w2. (!i. i < byte_width ==> byte_bit w1 i = byte_bit w2 i) ==> w1 = w2`;;
